lean-model/Klondike.lean
@@ -15,4 +15,5 @@ import Klondike.Initial
 import Klondike.Kills
 import Klondike.Restriction
 import Klondike.TwinSwap
+import Klondike.TwinExchange
 import Klondike.Frame
